simulation/correct_check_mem_aux2.v
@@ -2,7 +2,7 @@ From Coq Require Import List ZArith.
 Import ListNotations.
 From dx Require Import ResultMonad IR.
 From bpf.comm Require Import MemRegion Regs State Monad rBPFAST rBPFValues.
-From bpf.src Require Import DxNat DxIntegers DxValues DxMonad DxInstructions.
+From bpf.monadicmodel Require Import rBPFInterpreter.
 
 From compcert Require Import Coqlib Values Clight Memory Integers.
 
@@ -10,7 +10,7 @@ From bpf.clight Require Import interpreter.
 
 From bpf.proof Require Import MatchState Clightlogic clight_exec CommonLemma CorrectRel.
 
-From bpf.proof.correctproof Require Import correct_is_well_chunk_bool correct_get_sub correct_get_add correct_get_block_ptr correct_get_start_addr correct_get_block_size correct_get_block_perm.
+From bpf.simulation Require Import correct_is_well_chunk_bool correct_get_sub correct_get_add correct_get_block_ptr correct_get_start_addr correct_get_block_size correct_get_block_perm.
 
 Open Scope Z_scope.
 
@@ -22,8 +22,8 @@ Definition p : Clight.program := prog.
 (**r TODO: check_mem_aux2: memory_region -> perm -> addr -> chunk -> ptr *)
 
 (* [Args,Res] provides the mapping between the Coq and the C types *)
-Definition args  := [(memory_region:Type) ; (permission:Type); valu32_t; (AST.memory_chunk: Type)].
-Definition res  := valptr8_t.
+Definition args  := [(memory_region:Type) ; (permission:Type); val; (AST.memory_chunk: Type)].
+Definition res  := val.
 
 (* [f] is a Coq Monadic function with the right type *)
 Definition f := check_mem_aux2.
@@ -51,7 +51,7 @@ Definition match_arg  :
                         (DList.DNil _)))).
 
 Definition match_res (v1 :val) (v2:val) :=
-  v1 = v2 /\ ((exists b ofs, v1 = Vptr b ofs) \/ v1 = val32_zero).
+  v1 = v2 /\ ((exists b ofs, v1 = Vptr b ofs) \/ v1 = Vint (Int.zero)).
 
 
 Ltac build_app_aux T :=
@@ -172,18 +172,14 @@ Proof.
   correct_forward. 2:{ (**r if-else branch *)
   unfold correct_body.
   intros.
-  unfold Monad.returnM, val32_zero.
+  unfold Monad.returnM.
   unfold returnM.
   unfold Monad.returnM.
   intros.
-  exists (Vint Int.zero), m, Events.E0.
+  exists (Vint (Int.repr 0)), m, Events.E0.
   repeat split.
 
-  forward_star.
-  forward_star.
-  unfold Int.zero.
-  forward_star.
-  reflexivity.
+  repeat forward_star.
   intuition.
   constructor.
   reflexivity.
@@ -413,19 +409,19 @@ Proof.
   intuition eauto.
 
   unfold stateless, valu32_correct, memory_chunk_to_valu32, well_chunk_Z.
-  unfold stateless, match_chunk, memory_chunk_to_valu32, well_chunk_Z in H2.
+  unfold stateless, match_chunk, memory_chunk_to_valu32, well_chunk_Z in c4.
   intuition eauto.
   intros.
 
   (** goal: correct_body _ _ (if then else ... *)
 
   destruct (match x3 with
-  | Vint n2 => negb (Int.ltu n2 int32_0)
+  | Vint n2 => negb (Int.ltu n2 Int.zero)
   | _ => false
   end && compu_lt_32 x4 x1) eqn: Hcond1.
   destruct (compu_le_32 x3 (memory_chunk_to_valu32_upbound c2) &&
   match val32_modu x3 (memory_chunk_to_valu32 c2) with
-  | Vint n2 => Int.eq int32_0 n2
+  | Vint n2 => Int.eq Int.zero n2
   | _ => false
   end) eqn: Hcond2.
   (**r we have three goals: 
@@ -444,31 +440,30 @@ Proof.
         change B with B1
     end.
     unfold correct_body.
-    unfold returnM, val32_zero.
+    unfold returnM.
     intros.
 
     unfold INV0, INV in H.
-    get_invariant_more _hi_ofs.
-    get_invariant_more _lo_ofs.
-    get_invariant_more _size.
-    get_invariant_more _chunk.
-    get_invariant_more _ptr.
-    unfold correct_get_add.match_res, valu32_correct in H0.
-    destruct H0 as (H0_eq & (vi0 & Hvi0_eq)).
-    unfold correct_get_sub.match_res, valu32_correct in H2.
-    destruct H2 as (H2_eq & (vi2 & Hvi2_eq)).
-    unfold correct_get_block_size.match_res, valu32_correct in H4.
-    destruct H4 as (H4_eq & (vi4 & Hvi4_eq)).
-    unfold stateless, match_chunk, memory_chunk_to_valu32 in H6.
-    unfold correct_get_block_ptr.match_res, val_ptr_correct in H8.
-    destruct H8 as (H9_eq & (b & ofs & Hvi9_eq)).
+    get_invariant _hi_ofs.
+    get_invariant _lo_ofs.
+    get_invariant _size.
+    get_invariant _chunk.
+    get_invariant _ptr.
+    unfold correct_get_add.match_res, valu32_correct in c3.
+    destruct c3 as (H0_eq & (vi0 & Hvi0_eq)).
+    unfold correct_get_sub.match_res, valu32_correct in c4.
+    destruct c4 as (H2_eq & (vi2 & Hvi2_eq)).
+    unfold correct_get_block_size.match_res, valu32_correct in c5.
+    destruct c5 as (H4_eq & (vi4 & Hvi4_eq)).
+    unfold stateless, match_chunk, memory_chunk_to_valu32 in c6.
+    unfold correct_get_block_ptr.match_res, val_ptr_correct in c7.
+    destruct c7 as (H9_eq & (b & ofs & Hvi9_eq)).
     subst.
 
     exists (Vint Int.zero), m, Events.E0.
     repeat split.
 
     (**r we need the info given by Hcond1 *)
-    unfold int32_0 in Hcond1.
     assert (Hfalse: Int.ltu vi2 Int.zero = false). {
       unfold Int.ltu.
       rewrite Int.unsigned_zero. (**r Check zlt. *)
@@ -481,40 +476,23 @@ Proof.
     unfold negb in Hcond1; simpl in Hcond1.
 
 
-    forward_star.
-    repeat forward_star.
-    forward_star.
-    repeat forward_star. (**r Search (_ && _ = false).*)
+    forward_star. forward_star.
 
     simpl.
     fold Int.zero.
     rewrite Hfalse; simpl.
     reflexivity.
 
-    rewrite Int_eq_one_zero; simpl.
     forward_star.
-    repeat forward_star.
     simpl.
     rewrite Hcond1.
     reflexivity.
 
-    forward_star.
     repeat forward_star.
-    forward_star.
-    repeat forward_star.
-    rewrite Maps.PTree.gss.
+    right.
+    Transparent Archi.ptr64.
+    unfold Vnullptr.
     reflexivity.
-    rewrite Int.eq_true.
-    reflexivity.
-
-    forward_star.
-    repeat forward_star.
-    rewrite Int.eq_true; unfold negb.
-
-    forward_star.
-    forward_star.
-    reflexivity.
-    intuition.
 
     constructor; reflexivity.
   }
@@ -530,28 +508,27 @@ Proof.
         change B with B1
     end.
     unfold correct_body.
-    unfold returnM, val32_zero.
+    unfold returnM.
     intros.
 
     unfold INV0, INV in H.
-    get_invariant_more _hi_ofs.
-    get_invariant_more _lo_ofs.
-    get_invariant_more _size.
-    get_invariant_more _chunk.
-    get_invariant_more _ptr.
-    unfold correct_get_add.match_res, valu32_correct in H0.
-    destruct H0 as (H0_eq & (vi0 & Hvi0_eq)).
-    unfold correct_get_sub.match_res, valu32_correct in H2.
-    destruct H2 as (H2_eq & (vi2 & Hvi2_eq)).
-    unfold correct_get_block_size.match_res, valu32_correct in H4.
-    destruct H4 as (H4_eq & (vi4 & Hvi4_eq)).
-    unfold stateless, match_chunk, memory_chunk_to_valu32 in H6.
-    unfold correct_get_block_ptr.match_res, val_ptr_correct in H8.
-    destruct H8 as (H9_eq & (b & ofs & Hvi9_eq)).
+    get_invariant _hi_ofs.
+    get_invariant _lo_ofs.
+    get_invariant _size.
+    get_invariant _chunk.
+    get_invariant _ptr.
+    unfold correct_get_add.match_res, valu32_correct in c3.
+    destruct c3 as (H0_eq & (vi0 & Hvi0_eq)).
+    unfold correct_get_sub.match_res, valu32_correct in c4.
+    destruct c4 as (H2_eq & (vi2 & Hvi2_eq)).
+    unfold correct_get_block_size.match_res, valu32_correct in c5.
+    destruct c5 as (H4_eq & (vi4 & Hvi4_eq)).
+    unfold stateless, match_chunk, memory_chunk_to_valu32 in c6.
+    unfold correct_get_block_ptr.match_res, val_ptr_correct in c7.
+    destruct c7 as (H9_eq & (b & ofs & Hvi9_eq)).
     subst.
 
     (**r we need the info given by Hcond1, Hcond2 *)
-    unfold int32_0 in Hcond1, Hcond1.
     assert (Hfalse: Int.ltu vi2 Int.zero = false). {
       unfold Int.ltu.
       rewrite Int.unsigned_zero. (**r Check zlt. *)
@@ -591,7 +568,7 @@ Proof.
     exists (Vint Int.zero), m, Events.E0.
     repeat split.
 
-    unfold val32_modu, memory_chunk_to_valu32, Val.modu, int32_0 in Hcond2.
+    unfold val32_modu, memory_chunk_to_valu32, Val.modu in Hcond2.
     rewrite Hchunk_ne_zero in Hcond2.
 
     destruct (compu_le_32 (Vint vi2) (memory_chunk_to_valu32_upbound c2)) eqn: Heq1.
@@ -601,38 +578,14 @@ Proof.
     unfold compu_le_32, memory_chunk_to_valu32_upbound in Heq1.
     rewrite Int_max_unsigned_eq64 in Heq1.
 
-    forward_star.
-    repeat forward_star.
-    forward_star.
-    repeat forward_star.
+    forward_star. forward_star.
     simpl.
     rewrite Hfalse; reflexivity.
-    rewrite Int_eq_one_zero; unfold negb.
     forward_star.
-    repeat forward_star.
     simpl.
     rewrite Hcond1; reflexivity.
-    forward_star.
-    repeat forward_star.
-    forward_star.
-    repeat forward_star.
-    rewrite Maps.PTree.gss.
-    rewrite Int_eq_one_zero; reflexivity.
-    reflexivity.
-    forward_star.
-    repeat forward_star.
-    rewrite Int_eq_one_zero; unfold negb.
-    forward_star.
-    forward_star.
-    forward_star.
-    rewrite Maps.PTree.gso.
-    rewrite p1; reflexivity.
-    assumption.
-    rewrite Maps.PTree.gso.
-    rewrite p3; reflexivity.
-    assumption.
-    reflexivity.
-    reflexivity.
+    forward_star. forward_star.
+    forward_star. forward_star.
     simpl.
     unfold Int.sub; rewrite Int.unsigned_mone.
     rewrite He.
@@ -642,19 +595,10 @@ Proof.
     reflexivity.
 
     forward_star.
-    repeat forward_star.
-    rewrite Int_eq_one_zero; unfold negb.
-    repeat forward_star.
-    rewrite Maps.PTree.gso.
-    rewrite p1; reflexivity.
-    assumption.
-    rewrite Maps.PTree.gso.
-    rewrite p3; reflexivity.
-    assumption.
-    simpl.
 
 
     Transparent Archi.ptr64.
+    simpl.
     unfold Cop.sem_mod, Cop.sem_binarith, Cop.sem_cast; simpl.
 
     rewrite Hchunk_ne_zero.
@@ -665,64 +609,25 @@ Proof.
     rewrite Hcond2.
     reflexivity.
 
-    forward_star.
-    repeat forward_star.
-    forward_star.
-    repeat forward_star.
-    rewrite Maps.PTree.gss.
-    reflexivity.
-    reflexivity.
-    repeat rewrite Int.eq_true; unfold negb.
-    forward_star.
-    repeat forward_star.
-    forward_star.
-    reflexivity.
-
-    (**r if not lo_ofs <= 4294967295U - chunk then if 0U == lo_ofs % chunk then *)
-    unfold compu_le_32, memory_chunk_to_valu32_upbound in Heq1.
-    (**r Search (_ && _ = false).*)
-    forward_star.
-    repeat forward_star.
-    forward_star.
-    repeat forward_star.
+    forward_star. forward_star.
+    forward_star. forward_star.
+    forward_star. forward_star.
     simpl.
 
     rewrite Hfalse; unfold negb.
     reflexivity.
 
     forward_star.
-    repeat forward_star.
-    rewrite Int_eq_one_zero; unfold negb.
-    forward_star.
-    repeat forward_star.
     simpl.
     rewrite Hcond1;
     reflexivity.
 
-    forward_star.
-    repeat forward_star.
-    forward_star.
-    repeat forward_star.
-    rewrite Maps.PTree.gss.
-    reflexivity.
-    reflexivity.
-    repeat rewrite Int_eq_one_zero; unfold negb.
-
-    forward_star.
-    repeat forward_star.
-    forward_star.
-    repeat forward_star.
-    rewrite Maps.PTree.gso.
-    rewrite p1; reflexivity.
-    assumption.
-    rewrite Maps.PTree.gso.
-    rewrite p3; reflexivity.
-    assumption.
-    reflexivity.
-    reflexivity.
+    forward_star. forward_star.
+    forward_star. forward_star.
     simpl.
 
-    fold Int.mone.
+    (**r if not lo_ofs <= 4294967295U - chunk then if 0U == lo_ofs % chunk then *)
+    unfold compu_le_32, memory_chunk_to_valu32_upbound in Heq1.
     unfold Int.sub; rewrite Int.unsigned_mone.
     rewrite He.
 
@@ -730,22 +635,10 @@ Proof.
     rewrite Int_max_unsigned_eq64 in Heq1.
     rewrite Heq1.
     reflexivity.
-    rewrite Int.eq_true; unfold negb.
 
+    forward_star. forward_star.
+    forward_star. forward_star.
     forward_star.
-    repeat forward_star.
-    forward_star.
-    repeat forward_star.
-    forward_star.
-    repeat forward_star.
-    rewrite Maps.PTree.gss.
-    reflexivity.
-    reflexivity.
-    rewrite Int.eq_true; unfold negb.
-    forward_star.
-    repeat forward_star.
-    forward_star.
-    reflexivity.
     intuition.
     constructor; reflexivity.
   }
@@ -767,46 +660,40 @@ Proof.
     intros.
 
     unfold INV0, INV in H.
-    get_invariant_more _hi_ofs.
-    get_invariant_more _lo_ofs.
-    get_invariant_more _size.
-    get_invariant_more _chunk.
-    get_invariant_more _ptr.
-    get_invariant_more _perm.
-    get_invariant_more _mr_perm.
+    get_invariant _hi_ofs.
+    get_invariant _lo_ofs.
+    get_invariant _size.
+    get_invariant _chunk.
+    get_invariant _ptr.
+    get_invariant _perm.
+    get_invariant _mr_perm.
 
-    unfold correct_get_add.match_res, valu32_correct in H0.
-    destruct H0 as (H0_eq & (vi0 & Hvi0_eq)).
-    unfold correct_get_sub.match_res, valu32_correct in H2.
-    destruct H2 as (H2_eq & (vi2 & Hvi2_eq)).
-    unfold correct_get_block_size.match_res, valu32_correct in H4.
-    destruct H4 as (H4_eq & (vi4 & Hvi4_eq)).
-    unfold stateless, match_chunk, memory_chunk_to_valu32 in H6.
-    unfold correct_get_block_ptr.match_res, val_ptr_correct in H8.
-    destruct H8 as (H9_eq & (b & ofs & Hvi9_eq)).
-    unfold stateless, perm_correct in H10.
-    unfold correct_get_block_perm.match_res, perm_correct in H12.
+    unfold correct_get_add.match_res, valu32_correct in c3.
+    destruct c3 as (H0_eq & (vi0 & Hvi0_eq)).
+    unfold correct_get_sub.match_res, valu32_correct in c4.
+    destruct c4 as (H2_eq & (vi2 & Hvi2_eq)).
+    unfold correct_get_block_size.match_res, valu32_correct in c5.
+    destruct c5 as (H4_eq & (vi4 & Hvi4_eq)).
+    unfold stateless, match_chunk, memory_chunk_to_valu32 in c6.
+    unfold correct_get_block_ptr.match_res, val_ptr_correct in c7.
+    destruct c7 as (H9_eq & (b & ofs & Hvi9_eq)).
+    unfold stateless, perm_correct in c8.
+    unfold correct_get_block_perm.match_res, perm_correct in c9.
     subst.
 
     eexists; exists m, Events.E0.
     repeat split.
     Transparent Archi.ptr64.
-    forward_star.
-    repeat forward_star.
-    forward_star.
-    repeat forward_star.
+    forward_star. forward_star.
     simpl.
     rewrite andb_true_iff in Hcond1.
     destruct Hcond1 as (Hcond1 & _).
-    unfold int32_0, Int.zero in Hcond1.
+    unfold Int.zero in Hcond1.
     rewrite negb_true_iff in Hcond1.
     rewrite Hcond1.
     reflexivity.
 
-    rewrite Int_eq_one_zero.
-    unfold negb.
-    forward_star.
-    repeat forward_star.
+    forward_star. forward_star.
     simpl.
     rewrite andb_true_iff in Hcond1.
     destruct Hcond1 as (_ & Hcond1).
@@ -814,34 +701,8 @@ Proof.
     rewrite Hcond1.
     reflexivity.
 
-    forward_star.
-    repeat forward_star.
-    forward_star.
-    repeat forward_star.
-
-    rewrite Maps.PTree.gss.
-    rewrite Int_eq_one_zero.
-    reflexivity.
-
-    reflexivity.
-
-    rewrite Int_eq_one_zero.
-    unfold negb.
-    forward_star.
-    repeat forward_star.
-    forward_star.
-    repeat forward_star.
-    rewrite Maps.PTree.gso.
-    eauto.
-    unfold _lo_ofs, _t'9.
-    intro Hneq; inversion Hneq.
-    rewrite Maps.PTree.gso.
-    eauto.
-    unfold _chunk, _t'9.
-    intro Hneq; inversion Hneq.
-
-    reflexivity.
-    reflexivity.
+    forward_star. forward_star.
+    forward_star. forward_star.
     simpl.
     rewrite andb_true_iff in Hcond2.
     destruct Hcond2 as (Hcond2 & _).
@@ -860,18 +721,7 @@ Proof.
     rewrite Hcond2.
     reflexivity.
 
-    rewrite Int_eq_one_zero.
-    unfold negb.
-    forward_star.
-    repeat forward_star.
-    rewrite Maps.PTree.gso.
-    eauto.
-    unfold _lo_ofs, _t'9.
-    intro Hneq; inversion Hneq.
-    rewrite Maps.PTree.gso.
-    eauto.
-    unfold _chunk, _t'9.
-    intro Hneq; inversion Hneq.
+    forward_star. forward_star.
     simpl.
     unfold Cop.sem_mod, Cop.sem_binarith; simpl.
     assert (Hchunk_ne_zero: Int.eq (Int.repr (well_chunk_Z c2)) Int.zero = false). {
@@ -886,70 +736,27 @@ Proof.
     unfold Cop.sem_cast; simpl.
     rewrite andb_true_iff in Hcond2.
     destruct Hcond2 as (_ & Hcond2).
-    unfold val32_modu, memory_chunk_to_valu32, Val.modu, int32_0, Int.zero in Hcond2.
+    unfold val32_modu, memory_chunk_to_valu32, Val.modu,  Int.zero in Hcond2.
     destruct (Int.eq _ _) eqn: Hmodu; [inversion Hcond2 |].
     
     rewrite Hcond2.
     reflexivity.
 
-    forward_star.
-    repeat forward_star.
-    forward_star.
-    repeat forward_star.
-    rewrite Maps.PTree.gss.
-    rewrite Int_eq_one_zero.
-    reflexivity.
-    reflexivity.
-    forward_star.
-    repeat forward_star.
-    rewrite Int_eq_one_zero.
-    unfold negb.
-    forward_star.
-    repeat forward_star.
-    rewrite Maps.PTree.gso.
-    eauto.
-    rewrite Maps.PTree.gso.
-    eauto.
-    unfold _mr_perm, _t'9.
-    intro Hneq; inversion Hneq.
-    unfold _mr_perm, _t'8.
-    intro Hneq; inversion Hneq.
-    rewrite Maps.PTree.gso.
-    eauto.
-    rewrite Maps.PTree.gso.
-    eauto.
-    unfold _mr_perm, _t'9.
-    intro Hneq; inversion Hneq.
-    unfold _mr_perm, _t'8.
-    intro Hneq; inversion Hneq.
-    unfold Cop.sem_binary_operation, Cop.sem_cmp, Cop.sem_binarith; simpl.
-    unfold int32_0, int32_1, int32_2, int32_3, Int.one, Int.zero in *.
+    forward_star. forward_star.
+    forward_star. forward_star.
+    try post_process.
+
+    simpl.
+    unfold Cop.sem_cmp, Cop.sem_binarith; simpl.
     unfold Cop.sem_cast; simpl.
     unfold rBPFMemType.perm_ge in Hperm_ge.
-   destruct c0, x2; rewrite H10, H12; unfold Int.ltu; repeat rewrite Int_unsigned_repr_n; try reflexivity; try lia; simpl in Hperm_ge; inversion Hperm_ge.
+    destruct c0, x2; unfold Int.ltu; rewrite c8, c9; repeat rewrite Int_unsigned_repr_n; try reflexivity; try lia; simpl in Hperm_ge; inversion Hperm_ge.
 
     simpl.
     reflexivity.
-    rewrite Int_eq_one_zero.
-    unfold negb.
-    forward_star.
-    repeat forward_star.
-    rewrite Maps.PTree.gso.
-    eauto.
-    rewrite Maps.PTree.gso.
-    eauto.
-    unfold _ptr, _t'9.
-    intro Hneq; inversion Hneq.
-    unfold _ptr, _t'8.
-    intro Hneq; inversion Hneq.
-    rewrite Maps.PTree.gso.
-    eauto.
-    rewrite Maps.PTree.gso.
-    eauto.
-    unfold _lo_ofs, _t'9.
-    intro Hneq; inversion Hneq.
-    unfold _lo_ofs, _t'8.
-    intro Hneq; inversion Hneq.
+
+    forward_star. forward_star.
+    try post_process.
     reflexivity.
     reflexivity.
     simpl.
@@ -957,7 +764,6 @@ Proof.
     rewrite Ptrofs.mul_commut.
     rewrite Ptrofs.mul_one.
     forward_star.
-    reflexivity.
     left.
     eexists; eexists; reflexivity.
     simpl.
@@ -973,50 +779,44 @@ Proof.
         change B with B1
     end.
     unfold correct_body.
-    unfold returnM, Monad.returnM, valptr_null.
+    unfold returnM, Monad.returnM.
     intros.
 
     unfold INV0, INV in H.
-    get_invariant_more _hi_ofs.
-    get_invariant_more _lo_ofs.
-    get_invariant_more _size.
-    get_invariant_more _chunk.
-    get_invariant_more _ptr.
-    get_invariant_more _perm.
-    get_invariant_more _mr_perm.
+    get_invariant _hi_ofs.
+    get_invariant _lo_ofs.
+    get_invariant _size.
+    get_invariant _chunk.
+    get_invariant _ptr.
+    get_invariant _perm.
+    get_invariant _mr_perm.
 
-    unfold correct_get_add.match_res, valu32_correct in H0.
-    destruct H0 as (H0_eq & (vi0 & Hvi0_eq)).
-    unfold correct_get_sub.match_res, valu32_correct in H2.
-    destruct H2 as (H2_eq & (vi2 & Hvi2_eq)).
-    unfold correct_get_block_size.match_res, valu32_correct in H4.
-    destruct H4 as (H4_eq & (vi4 & Hvi4_eq)).
-    unfold stateless, match_chunk, memory_chunk_to_valu32 in H6.
-    unfold correct_get_block_ptr.match_res, val_ptr_correct in H8.
-    destruct H8 as (H9_eq & (b & ofs & Hvi9_eq)).
-    unfold stateless, perm_correct in H10.
-    unfold correct_get_block_perm.match_res, perm_correct in H12.
+    unfold correct_get_add.match_res, valu32_correct in c3.
+    destruct c3 as (H0_eq & (vi0 & Hvi0_eq)).
+    unfold correct_get_sub.match_res, valu32_correct in c4.
+    destruct c4 as (H2_eq & (vi2 & Hvi2_eq)).
+    unfold correct_get_block_size.match_res, valu32_correct in c5.
+    destruct c5 as (H4_eq & (vi4 & Hvi4_eq)).
+    unfold stateless, match_chunk, memory_chunk_to_valu32 in c6.
+    unfold correct_get_block_ptr.match_res, val_ptr_correct in c7.
+    destruct c7 as (H9_eq & (b & ofs & Hvi9_eq)).
+    unfold stateless, perm_correct in c8.
+    unfold correct_get_block_perm.match_res, perm_correct in c9.
     subst.
 
     eexists; exists m, Events.E0.
     repeat split.
-    forward_star.
-    repeat forward_star.
-    forward_star.
-    repeat forward_star.
+    forward_star. forward_star.
     simpl.
 
     rewrite andb_true_iff in Hcond1.
     destruct Hcond1 as (Hcond1 & _).
-    unfold int32_0, Int.zero in Hcond1.
+    unfold  Int.zero in Hcond1.
     rewrite negb_true_iff in Hcond1.
     rewrite Hcond1.
     reflexivity.
 
-    rewrite Int_eq_one_zero.
-    unfold negb.
     forward_star.
-    repeat forward_star.
     simpl.
     rewrite andb_true_iff in Hcond1.
     destruct Hcond1 as (_ & Hcond1).
@@ -1024,37 +824,10 @@ Proof.
     rewrite Hcond1.
     reflexivity.
 
-    forward_star.
-    repeat forward_star.
-    forward_star.
-    repeat forward_star.
+    forward_star. forward_star.
+    forward_star. forward_star.
 
-    rewrite Maps.PTree.gss.
-    rewrite Int_eq_one_zero.
-    reflexivity.
-
-    reflexivity.
-
-    rewrite Int_eq_one_zero.
-    unfold negb.
-    forward_star.
-    repeat forward_star.
-    forward_star.
-    repeat forward_star.
-    rewrite Maps.PTree.gso.
-    eauto.
-    unfold _lo_ofs, _t'9.
-    intro Hneq; inversion Hneq.
-    rewrite Maps.PTree.gso.
-    eauto.
-    unfold _chunk, _t'9.
-    intro Hneq; inversion Hneq.
-
-    reflexivity.
-    reflexivity.
     simpl.
-    rewrite andb_true_iff in Hcond2.
-    destruct Hcond2 as (Hcond2 & _).
     unfold compu_le_32, memory_chunk_to_valu32_upbound in Hcond2.
     unfold Int.sub.
     assert (Hwell_chunk_unsigned: Int.unsigned (Int.repr (well_chunk_Z c2)) = well_chunk_Z c2). {
@@ -1067,21 +840,12 @@ Proof.
     assert (Heq: two_power_nat 32 - 1 = 4294967295). { reflexivity. }
     rewrite Heq; clear Heq.
     rewrite Int_max_unsigned_eq64 in Hcond2.
+    rewrite andb_true_iff in Hcond2.
+    destruct Hcond2 as (Hcond2 & _).
     rewrite Hcond2.
     reflexivity.
 
-    rewrite Int_eq_one_zero.
-    unfold negb.
     forward_star.
-    repeat forward_star.
-    rewrite Maps.PTree.gso.
-    eauto.
-    unfold _lo_ofs, _t'9.
-    intro Hneq; inversion Hneq.
-    rewrite Maps.PTree.gso.
-    eauto.
-    unfold _chunk, _t'9.
-    intro Hneq; inversion Hneq.
     simpl.
     unfold Cop.sem_mod, Cop.sem_binarith; simpl.
     assert (Hchunk_ne_zero: Int.eq (Int.repr (well_chunk_Z c2)) Int.zero = false). {
@@ -1096,299 +860,32 @@ Proof.
     unfold Cop.sem_cast; simpl.
     rewrite andb_true_iff in Hcond2.
     destruct Hcond2 as (_ & Hcond2).
-    unfold val32_modu, memory_chunk_to_valu32, Val.modu, int32_0, Int.zero in Hcond2.
+    unfold val32_modu, memory_chunk_to_valu32, Val.modu,  Int.zero in Hcond2.
     destruct (Int.eq _ _) eqn: Hmodu; [inversion Hcond2 |].
     
     rewrite Hcond2.
     reflexivity.
 
+    forward_star. forward_star.
     forward_star.
-    repeat forward_star.
-    forward_star.
-    repeat forward_star.
-    rewrite Maps.PTree.gss.
-    rewrite Int_eq_one_zero.
-    reflexivity.
-    reflexivity.
-    forward_star.
-    repeat forward_star.
-    rewrite Int_eq_one_zero.
-    unfold negb.
-    forward_star.
-    repeat forward_star.
-    rewrite Maps.PTree.gso.
-    eauto.
-    rewrite Maps.PTree.gso.
-    eauto.
-    unfold _mr_perm, _t'9.
-    intro Hneq; inversion Hneq.
-    unfold _mr_perm, _t'8.
-    intro Hneq; inversion Hneq.
-    rewrite Maps.PTree.gso.
-    eauto.
-    rewrite Maps.PTree.gso.
-    eauto.
-    unfold _mr_perm, _t'9.
-    intro Hneq; inversion Hneq.
-    unfold _mr_perm, _t'8.
-    intro Hneq; inversion Hneq.
-    unfold Cop.sem_binary_operation, Cop.sem_cmp, Cop.sem_binarith; simpl.
-    unfold int32_0, int32_1, int32_2, int32_3, Int.one, Int.zero in *.
+    post_process.
+    post_process.
+    simpl.
+    unfold Cop.sem_cmp, Cop.sem_binarith; simpl.
     unfold Cop.sem_cast; simpl.
     unfold rBPFMemType.perm_ge in Hperm_ge.
-   destruct c0, x2; rewrite H10, H12; unfold Int.ltu; repeat rewrite Int_unsigned_repr_n; try reflexivity; try lia; simpl in Hperm_ge; inversion Hperm_ge.
+    destruct c0 eqn: Hc0_eq; destruct x2 eqn: Hx2_eq; inversion Hperm_ge; rewrite c8, c9; unfold Int.ltu; repeat rewrite Int_unsigned_repr_n; try reflexivity; try lia; simpl in Hperm_ge; inversion Hperm_ge.
 
-    admit. (**r TODO *)
     simpl.
     reflexivity.
-    admit.
-    rewrite Int_eq_one_zero.
-    unfold negb.
-    forward_star.
-    repeat forward_star.
-    rewrite Maps.PTree.gso.
-    eauto.
-    rewrite Maps.PTree.gso.
-    eauto.
-    unfold _ptr, _t'9.
-    intro Hneq; inversion Hneq.
-    unfold _ptr, _t'8.
-    intro Hneq; inversion Hneq.
-    rewrite Maps.PTree.gso.
-    eauto.
-    rewrite Maps.PTree.gso.
-    eauto.
-    unfold _lo_ofs, _t'9.
-    intro Hneq; inversion Hneq.
-    unfold _lo_ofs, _t'8.
-    intro Hneq; inversion Hneq.
-    reflexivity.
-    reflexivity.
-    simpl.
-    fold Ptrofs.one.
-    rewrite Ptrofs.mul_commut.
-    rewrite Ptrofs.mul_one.
-    forward_star.
-    reflexivity.
-    left.
-    eexists; eexists; reflexivity.
-    simpl.
-    constructor.
 
-    reflexivity.
-
-  
-
-  eapply correct_statement_seq_body_unit.
-  change_app_for_statement.
-  (**r goal: correct_statement p unit (app f a) fn (Scall None (Evar ... *)
-  eapply correct_statement_call_none.
-  TODO.
-  unfold list_rel_arg,app;
-  match goal with
-  |- correct_body _ _ _ _ ?B _ ?INV
-               _ _ _ _ =>
-    let I := fresh "INV" in
-    set (I := INV) ; simpl in I;
-    let B1 := eval simpl in B in
-      change B with B1
-  end.
-  unfold correct_body.
-  intro.
-  destruct (returnM (Val.add x x2) st5) eqn: Hreturn; [idtac | constructor].
-  unfold returnM in Hreturn.
-  destruct p0.
-  intros.
-
-  (**r we need the value of those vairable in the memory, they will be used later *)
-  unfold INV0, INV in H.
-  get_invariant_more _hi_ofs.
-  get_invariant_more _lo_ofs.
-  get_invariant_more _size.
-  get_invariant_more _chunk.
-  get_invariant_more _ptr.
-  unfold correct_get_add.match_res, valu32_correct in H0.
-  destruct H0 as (H0_eq & (vi0 & Hvi0_eq)).
-  unfold correct_get_sub.match_res, valu32_correct in H2.
-  destruct H2 as (H2_eq & (vi2 & Hvi2_eq)).
-  unfold correct_get_block_size.match_res, valu32_correct in H4.
-  destruct H4 as (H4_eq & (vi4 & Hvi4_eq)).
-  unfold stateless, match_chunk, memory_chunk_to_valu32 in H6.
-  unfold correct_get_block_ptr.match_res, val_ptr_correct in H8.
-  destruct H8 as (H9_eq & (b & ofs & Hvi9_eq)).
-  subst.
-
-  exists (Val.add (Vptr b ofs) (Vint vi2)), m, Events.E0.
-  repeat split.
-  + 
+    forward_star. forward_star.
+    right.
     Transparent Archi.ptr64.
-    forward_star.
-    repeat forward_star.
-    forward_star.
-    repeat forward_star.
-    unfold Cop.bool_val, Val.of_bool, Cop.sem_cmp, Cop.sem_binarith, Cop.sem_cast; simpl.
-    unfold Int.ltu.
-    fold Int.zero.
-    rewrite Int.unsigned_zero.
-    assert (Hvi3_ge: ((Int.unsigned vi2) >= 0)%Z). {
-      assert (Hhi_range: (0 <= Int.unsigned vi2 <= Int.max_unsigned)%Z).
-      apply Int.unsigned_range_2.
-      lia.
-    }
-    rewrite zlt_false; simpl.
-    rewrite Int_eq_one_zero; reflexivity.
-    assumption.
-
-    (** Smallstep.star _ _ (State _ (if negb false ... *)
-    simpl.
-    forward_star.
-    forward_star.
-    unfold Cop.sem_cast, Val.of_bool; simpl.
-    apply andb_prop in Hcond1.
-    destruct Hcond1 as (Hcond1_1 & Hcond1_2).
-    unfold compu_lt_32 in Hcond1_2.
-    rewrite Hcond1_2; simpl.
-    rewrite Int_eq_one_zero; reflexivity.
-    forward_star.
-    repeat forward_star.
-    forward_star.
-    repeat forward_star.
-    rewrite Maps.PTree.gss; reflexivity.
+    unfold Vnullptr.
     reflexivity.
-    (** Smallstep.star _ _(State _ (if negb (Int.eq Int.one Int.zero) then ... *)
-    forward_star.
-    rewrite Int_eq_one_zero.
-    unfold negb.
-    repeat forward_star.
-
-    (**r after we need the info about Hcond2, I do it here*)
-    apply andb_prop in Hcond2.
-    destruct Hcond2 as (Hcond2_1 & Hcond2_2).
-    unfold compu_le_32, memory_chunk_to_valu32_upbound in Hcond2_1.
-    rewrite Int_max_unsigned_eq64 in Hcond2_1.
-    unfold val32_modu, Val.modu, memory_chunk_to_valu32 in Hcond2_2.
-    
-    destruct (Int.eq (Int.repr (well_chunk_Z c1)) Int.zero) eqn: Heq_zero; try discriminate.
-
-    (**r we also need those info below *)
-    assert (Hneq1: _lo_ofs <> _t'8). {
-      unfold _lo_ofs, _t'8.
-      intro Hneq; inversion Hneq.
-    }
-    assert (Hneq2: _chunk <> _t'8). {
-      unfold _chunk, _t'8.
-      intro Hneq; inversion Hneq.
-    }
-
-    forward_star.
-    forward_star.
-    (**r the 1st place I need _lo_ofs & _chunk *)
-    apply Maps.PTree.gso with (x:=Vint Int.one) (m:=le5) in Hneq1.
-    rewrite Hneq1.
-    rewrite p1; reflexivity.
-    apply Maps.PTree.gso with (x:=Vint Int.one) (m:=le5) in Hneq2.
-    rewrite Hneq2.
-    rewrite p3; reflexivity.
-    reflexivity.
-    reflexivity.
-    unfold Cop.bool_val, Val.of_bool; simpl.
-
-    (**the first place I need Hcond2 *)
-    fold Int.mone.
-    unfold Int.sub; rewrite Int.unsigned_mone.
-    assert (He: Int.modulus - 1 = 4294967295). {
-      unfold Int.modulus, Int.wordsize, Wordsize_32.wordsize; reflexivity.
-    }
-    rewrite He.
-
-    assert (Hwell_chunk_unsigned: Int.unsigned (Int.repr (well_chunk_Z c1)) = well_chunk_Z c1). {
-      destruct c1; simpl; try (fold Int.zero; apply Int.unsigned_zero); try rewrite Int.unsigned_repr; try reflexivity; try rewrite Int_max_unsigned_eq64; try lia.
-    }
-    rewrite Hwell_chunk_unsigned.
-    rewrite Hcond2_1; simpl.
-    rewrite Int_eq_one_zero; unfold negb; reflexivity.
-    Search (if true then _ else _).
-    match goal with
-    | |- context[if true then ?X else ?Y] =>
-        change (if true then X else Y) with X
-    end.
-
-    forward_star.
-    forward_star.
-    (**r the 2nd place I need _lo_ofs & _chunk *)
-    apply Maps.PTree.gso with (x:=Vint Int.one) (m:=le5) in Hneq1.
-    rewrite Hneq1.
-    rewrite p1; reflexivity.
-    apply Maps.PTree.gso with (x:=Vint Int.one) (m:=le5) in Hneq2.
-    rewrite Hneq2.
-    rewrite p3; reflexivity.
-
-    unfold Cop.sem_binary_operation; simpl.
-    unfold Cop.sem_mod, Cop.sem_binarith; simpl.
-    (**r here we need to prove `modu`, i.e. (well_chunk_Z c1) <> 0, we should see the Hypothesis `Hcond2` *)
-    rewrite Heq_zero;
-    reflexivity.
-    reflexivity.
-
-    unfold Cop.bool_val, Val.of_bool; simpl.
-    unfold int32_0, Int.zero in Hcond2_2.
-    rewrite Hcond2_2.
-    reflexivity.
-
-    forward_star.
-    repeat forward_star.
-    forward_star.
-    repeat forward_star.
-    rewrite Maps.PTree.gss.
-    rewrite Int_eq_one_zero.
-    reflexivity.
-    reflexivity.
-
-    rewrite Int_eq_one_zero; unfold negb.
-    forward_star.
-    repeat forward_star.
-
-    assert (Hneq3: _ptr <> _t'7). {
-      unfold _ptr, _t'7.
-      intro Hneq; inversion Hneq.
-    }
-    assert (Hneq4: _ptr <> _t'8). {
-      unfold _ptr, _t'8.
-      intro Hneq; inversion Hneq.
-    }
-    apply Maps.PTree.gso with (x:=Vint Int.one) (m:=(Maps.PTree.set _t'8 (Vint Int.one) le5)) in Hneq3; rewrite Hneq3.
-    apply Maps.PTree.gso with (x:=Vint Int.one) (m:=le5) in Hneq4; rewrite Hneq4.
-    rewrite p4; reflexivity.
-
-    assert (Hneq3: _lo_ofs <> _t'7). {
-      unfold _lo_ofs, _t'7.
-      intro Hneq; inversion Hneq.
-    }
-    apply Maps.PTree.gso with (x:=Vint Int.one) (m:=(Maps.PTree.set _t'8 (Vint Int.one) le5)) in Hneq3; rewrite Hneq3.
-    apply Maps.PTree.gso with (x:=Vint Int.one) (m:=le5) in Hneq1; rewrite Hneq1.
-    rewrite p1; reflexivity.
-    unfold Cop.sem_binary_operation, Cop.sem_add, Cop.classify_add; simpl.
-    reflexivity.
-    reflexivity.
-
-    unfold Ptrofs.mul, Ptrofs.of_intu.
-    assert (Hofs_one: Ptrofs.unsigned (Ptrofs.repr 1) = 1). {
-      apply Ptrofs.unsigned_repr.
-      rewrite Ptrofs_max_unsigned_eq32.
-      lia.
-    }
-    rewrite Hofs_one.
-    rewrite Z.mul_1_l.
-    rewrite Ptrofs.repr_unsigned.
     constructor.
-    reflexivity.
-  + inversion Hreturn.
-    reflexivity.
-  + inversion Hreturn.
-    left; exists b, (Ptrofs.add ofs (Ptrofs.of_int vi2)).
-    reflexivity.
-  + constructor.
-  + inversion Hreturn.
+
     reflexivity.
 Qed.
 
